io/Free.fst
@@ -36,7 +36,7 @@ let req_sig : op_sig req_cmds = { args = req_args; res = req_res; }
 
 noeq
 type free (op:Type0) (s:op_sig op) (a:Type u#a) : Type u#(max 1 a)=
-| Call : (l:op) -> (arg:s.args l) -> cont:(s.res l arg -> free u#a op s a) -> free op s a
+| Call : (trusted:bool) -> (l:op) -> (arg:s.args l) -> cont:(s.res l arg -> free u#a op s a) -> free op s a
 | PartialCall : (pre:pure_pre) -> cont:((squash pre) -> free u#a op s a) -> free op s a
 | Return : a -> free op s a
 
@@ -53,8 +53,8 @@ let rec free_bind
   free op s b =
   match l with
   | Return x -> k x
-  | Call cmd args fnc ->
-      Call cmd args (fun i ->
+  | Call tr cmd args fnc ->
+      Call tr cmd args (fun i ->
         free_bind op s a b (fnc i) k)
   | PartialCall pre fnc ->
       PartialCall pre (fun _ ->
